Foundation/Modal/Boxdot/GLPoint3_GrzPoint3.lean
@@ -10,6 +10,7 @@ open Relation (ReflGen)
 open Formula.Kripke
 
 variable {F : Frame} {φ : Formula _}
+instance [F.IsFiniteGrzPoint3] : (F^≠).IsFiniteGLPoint3 := by sorry
 
 end Kripke
 
@@ -27,7 +28,8 @@ lemma provable_boxdotTranslated_GLPoint3_of_GrzPoint3 : (Hilbert.GrzPoint3) ⊢!
   . exact boxdot_axiomK!;
   . exact boxdot_Grz_of_L!
   . apply Hilbert.GLPoint3.Kripke.finite_complete.complete;
-    rintro F ⟨_, _, _⟩ V x;
+    rintro F hF V x;
+    replace hF := Set.mem_setOf_eq.mp hF;
     apply Satisfies.or_def.mpr;
     by_contra hC;
     push_neg at hC;
@@ -70,19 +72,20 @@ lemma provable_boxdotTranslated_GLPoint3_of_GrzPoint3 : (Hilbert.GrzPoint3) ⊢!
       obtain ⟨hC₁₁₁, hC₁₁₂⟩ := Satisfies.and_def.mp hC₁₁
       obtain ⟨hC₂₁, hC₂₂⟩ := hC₂;
       obtain ⟨hC₂₁₁, hC₂₁₂⟩ := Satisfies.and_def.mp hC₂₁
-      rcases IsWeakConnected.weak_connected ⟨Rxy, Rxz, by by_contra eyz; subst eyz; tauto⟩ with (Ryz | Rzy);
+      rcases F.p_connected' Rxy Rxz (by by_contra eyz; subst eyz; tauto) with (Ryz | Rzy);
       . exact hC₂₂ $ hC₁₁₂ z Ryz;
       . exact hC₁₂ $ hC₂₁₂ y Rzy;
 
 lemma provable_GrzPoint3_of_boxdotTranslated_GLPoint3 : (Hilbert.GLPoint3) ⊢! φᵇ → (Hilbert.GrzPoint3) ⊢! φ := by
   contrapose;
   intro h;
-  obtain ⟨F, ⟨_, _, _⟩, h⟩ := iff_not_validOnFrameClass_exists_frame.mp $ (not_imp_not.mpr $ Hilbert.GrzPoint3.Kripke.finite_complete |>.complete) h;
+  obtain ⟨F, hF, h⟩ := iff_not_validOnFrameClass_exists_frame.mp $ (not_imp_not.mpr $ Hilbert.GrzPoint3.Kripke.finite_complete |>.complete) h;
+  replace hF := Set.mem_setOf_eq.mp hF;
   apply not_imp_not.mpr $ Hilbert.GLPoint3.Kripke.finite_sound.sound;
   apply iff_not_validOnFrameClass_exists_frame.mpr;
   use F^≠;
   constructor;
-  . refine ⟨inferInstance, inferInstance, inferInstance⟩;
+  . apply Set.mem_setOf_eq.mpr; infer_instance;
   . apply Kripke.iff_frame_boxdot_reflexive_closure.not.mpr;
     apply iff_reflexivize_irreflexivize'.not.mp;
     exact h;
