Foundation/Modal/Kripke/Antisymmetric.lean
@@ -1,5 +1,4 @@
 import Foundation.Modal.Kripke.AxiomGeach
-import Foundation.Modal.Kripke.Closure
 
 
 namespace LO.Modal
@@ -13,12 +12,7 @@ protected abbrev Frame.IsAntisymmetric (F : Frame) := IsAntisymm _ F.Rel
 
 lemma Frame.antisymm [F.IsAntisymmetric] : ∀ {x y : F.World}, x ≺ y → y ≺ x → x = y := by apply IsAntisymm.antisymm
 
-
-protected abbrev Frame.IsPartialOrder (F : Frame) := IsPartialOrder _ F.Rel
-
-instance [F.IsPartialOrder] : F.IsReflexive := by simp
-instance [F.IsPartialOrder] : F.IsTransitive := by simp
-instance [F.IsPartialOrder] : F.IsAntisymmetric := ⟨by apply Frame.antisymm⟩
+protected class Frame.IsPartialOrder (F : Frame) extends F.IsReflexive, F.IsTransitive, F.IsAntisymmetric
 
 end Kripke
 
