Foundation/Modal/Kripke/Irreflexivize.lean
@@ -1,0 +1,35 @@
+import Foundation.Modal.Kripke.Irreflexive
+
+namespace LO.Modal.Kripke
+
+namespace Frame
+
+variable {F : Frame} {x y z : F.World}
+
+abbrev IrreflRel := F.Rel.IrreflGen
+infix:50 " ≺^≠ " => IrreflRel
+
+abbrev IrreflGen (F : Frame) : Frame := ⟨F.World, (· ≺^≠ ·)⟩
+postfix:95 "^≠" => IrreflGen
+
+namespace IrreflGen
+
+instance : Coe (F.World) (F^≠.World) := ⟨id⟩
+
+instance [Finite F] : Finite (F^≠) := inferInstance
+instance [F.IsFinite] : (F^≠).IsFinite := inferInstance
+
+instance : (F^≠).IsIrreflexive := ⟨IsIrrefl.irrefl⟩
+
+instance [F.IsIrreflexive] [F.IsTransitive] : (F^≠).IsTransitive := by simp
+
+instance [F.IsAntisymmetric] : F^≠.IsAntisymmetric := ⟨by
+  rintro x y ⟨_, Rxy⟩ ⟨_, Ryx⟩;
+  exact F.antisymm Rxy Ryx;
+⟩
+
+end IrreflGen
+
+end Frame
+
+end LO.Modal.Kripke
