Foundation/Propositional/Kripke/Filtration.lean
@@ -1,5 +1,4 @@
 import Mathlib.Data.Set.Finite.Powerset
-import Foundation.Vorspiel.Relation.Iterate
 import Foundation.Propositional.Kripke.Preservation
 
 universe u v
